lib/Base/LinearOption.i.dfy
@@ -1,16 +1,39 @@
-module LinearOption {
-  linear datatype lOption<V> = lNone | lSome(linear value: V)
+include "Option.s.dfy"
 
-  function MapLOption<V0, V1>(opt: lOption<V0>, f: V0 ~> V1) :
-    (result: lOption<V1>)
-  requires opt.lSome? ==> f.requires(opt.value)
-  ensures opt.lSome? <==> result.lSome?
-  ensures result.lSome? ==> result.value == f(opt.value)
-  reads if opt.lSome? then f.reads(opt.value) else {}
+module LinearOption {
+  import opened Options
+
+  linear datatype TupleResult<V> = TupleResult(linear result: lOption<V>, linear other: lOption<V>)
+
+  linear datatype lOption<V> = lNone | lSome(linear value: V)
   {
-    match opt {
-      case lSome(v) => lSome(f(v))
-      case lNone => lNone
+    function Map<V1>(f: V ~> V1) : (result: lOption<V1>)
+    requires this.lSome? ==> f.requires(this.value)
+    ensures this.lSome? <==> result.lSome?
+    ensures result.lSome? ==> result.value == f(this.value)
+    reads if this.lSome? then f.reads(this.value) else {}
+    {
+      match this {
+        case lSome(v) => lSome(f(v))
+        case lNone => lNone
+      }
     }
+
+    function Option() : (result: Option<V>)
+    {
+      match this {
+        case lSome(v) => Some(v)
+        case lNone => None
+      }
+    }
+  }
+}
+
+module Test {
+  import opened LinearOption
+  function Something(a: lOption<int>): lOption<int>
+  ensures a.lSome? ==> Something(a).lSome? && Something(a).value == a.value * 2
+  {
+    a.Map(x => x * 2)
   }
 }
