lib/Base/sequences.i.dfy
@@ -20,6 +20,11 @@ module Sequences {
     run[|run|-1]
   }
 
+  function FirstOpt<E>(run: seq<E>) : Option<E>
+  {
+    if |run| == 0 then None else Some(run[0])
+  }
+
   function DropLast<E>(run: seq<E>) : seq<E>
     requires |run| > 0;
   {
@@ -120,6 +125,29 @@ module Sequences {
   ensures forall i | pos <= i < |s| - 1 :: remove(s, pos)[i] == s[i+1]
   {
     s[.. pos] + s[pos + 1 ..]
+  }
+
+  function {:opaque} RemoveValue<V>(s: seq<V>, v: V) : seq<V>
+  // ensures forall i: nat | i < |RemoveValue(s, v)| :: RemoveValue(s, v)[i] != v
+  ensures Set(RemoveValue(s, v)) == Set(s) - {v}
+  {
+    if s == [] then s
+      else (if s[0] == v then [] else [s[0]]) + RemoveValue(s[1..], v)
+  }
+
+  lemma RemoveValueMultiset<V>(s: seq<V>, v: V) returns (res: seq<V>)
+  ensures Set(RemoveValue(s, v)) == Set(s) - {v}
+  {
+    reveal_RemoveValue();
+    if s == [] {
+      assert Set(RemoveValue(s, v)) == Set(s) - {v};
+    } else {
+      assert s == [s[0]] + s[1..];
+      var _ := RemoveValueMultiset(s[1..], v);
+      assert Set(s) == Set([s[0]]) + Set(s[1..]);
+      // TODO(andreal)
+      assume Set(RemoveValue(s, v)) == Set(s) - {v};
+    }
   }
 
   function {:opaque} insert<A>(s: seq<A>, a: A, pos: int) : seq<A>
